Regex/Nfa.lean
@@ -1,3 +1,4 @@
+import Std.Data.Fin.Basic
 import Regex.Utils
 
 namespace NFA
@@ -6,33 +7,11 @@ namespace NFA
 ## NFA
 
 A byte oriented [Thompson](https://en.wikipedia.org/wiki/Thompson%27s_construction)
-non-deterministic finite automaton (`NFA`).
+non-deterministic finite automaton (`Checked.NFA`).
 -/
-
-/-- The identifier of a finite automaton state, represented by a Nat -/
-abbrev StateID := Nat
 
 /-- The identifier of a regex pattern, represented by a Nat -/
 abbrev PatternID := Nat
-
-/-- A single transition to another state.
-    This transition may only be followed if the current char in the haystack
-    falls in the inclusive range of chars specified. -/
-structure Transition where
-  /-- The inclusive start of the char range. -/
-  start: UInt32
-  /-- The inclusive end of the char range. -/
-  «end»: UInt32
-  /--  The identifier of the state to transition to. -/
-  next: StateID
-
-namespace Transition
-
-/-- check if `c` falls in the inclusive range of chars specified in Transition `trans` -/
-def «matches» (trans : Transition) (c : Char) : Bool :=
-  trans.start <= c.val && c.val <= trans.end
-
-end Transition
 
 /-- The high-level intermediate representation for a look-around assertion. -/
 inductive Look where
@@ -80,6 +59,31 @@ end Look
 
 instance : ToString Look where
   toString := Look.toString
+
+namespace Unchecked
+
+/-- The identifier of a finite automaton state, represented by a Nat.
+    The identifier may refer to a non existing state. -/
+abbrev StateID := Nat
+
+/-- A single transition to another state.
+    This transition may only be followed if the current char in the haystack
+    falls in the inclusive range of chars specified. -/
+structure Transition where
+  /-- The inclusive start of the char range. -/
+  start: UInt32
+  /-- The inclusive end of the char range. -/
+  «end»: UInt32
+  /--  The identifier of the state to transition to. -/
+  next: StateID
+
+namespace Transition
+
+/-- check if `c` falls in the inclusive range of chars specified in Transition `trans` -/
+def «matches» (trans : Transition) (c : Char) : Bool :=
+  trans.start <= c.val && c.val <= trans.end
+
+end Transition
 
 /-- A state in an NFA. -/
 inductive State where
@@ -156,5 +160,155 @@ def toString (nfa : NFA) : String :=
 
 end NFA
 
+end Unchecked
+
+instance : ToString Unchecked.NFA where
+  toString := Unchecked.NFA.toString
+
+namespace Checked
+
+/-- A single transition to another state.
+    This transition may only be followed if the current char in the haystack
+    falls in the inclusive range of chars specified. -/
+structure Transition (n : Nat) where
+  /-- The inclusive start of the char range. -/
+  start: UInt32
+  /-- The inclusive end of the char range. -/
+  «end»: UInt32
+  /--  The identifier of the state to transition to. -/
+  next: Fin n
+
+namespace Transition
+
+/-- check if `c` falls in the inclusive range of chars specified in Transition `trans` -/
+def «matches» (trans : Transition n) (c : Char) : Bool :=
+  trans.start <= c.val && c.val <= trans.end
+
+end Transition
+
+/-- A state in an NFA, the elements of `Fin n` refer to existing states in the NFA. -/
+inductive State (n : Nat) where
+  /-- An empty state whose only purpose is to forward the automaton to
+      another state via an unconditional epsilon transition. -/
+  | Empty (next: Fin n) : State n
+  /-- A state with a single transition that can only be taken if the current
+      input symbol is in a particular range of chars. -/
+  | ByteRange (trans : Transition n) : State n
+  /-- A sequence of transitions used to represent a sparse state. -/
+  | SparseTransitions (transitions : Array $ Transition n) : State n
+  /-- A conditional epsilon transition satisfied via some sort of look-around.  -/
+  | Look (look : Look) (next: Fin n) : State n
+  /--An alternation such that there exists an epsilon transition to all states in `alternates`,
+     where matches found via earlier transitions are preferred over later transitions. -/
+  | Union (alternates: Array $ Fin n) : State n
+  /--An alternation such that there exists an epsilon transition to all states in `alternates`,
+     where matches found via later transitions are preferred over earlier transitions. -/
+  | UnionReverse (alternates: Array $ Fin n) : State n
+  /-- An alternation such that there exists precisely two unconditional epsilon transitions -/
+  | BinaryUnion (alt1: Fin n) (alt2: Fin n) : State n
+  /-- An empty state that records a capture location.
+      `slot` in this context refers to the specific capture group slot
+       offset that is being recorded. Each capturing group has two slots
+       corresponding to the start and end of the matching portion of that
+       group. -/
+  | Capture (next: Fin n) (pattern_id: PatternID) (group_index: Nat) (slot: Nat) : State n
+  /-- A match state. There is at least one such occurrence of this state for
+      each regex that can match that is in this NFA. -/
+  | Match (pattern_id : PatternID) : State n
+
+namespace State
+
+def toString : State n -> String
+  | .Empty next => s!"Empty => {next}"
+  | .ByteRange trans =>
+      s!"byte-range {intAsString trans.start}-{intAsString trans.end} => {trans.next}"
+  | .SparseTransitions trans =>
+      let lines := String.join (trans.toList |> List.map (fun t =>
+            s!" {intAsString t.start}-{intAsString t.end} => {t.next}"))
+      s!"SparseTransitions [{lines} ]"
+  | .Look look next =>
+      s!"Look {look} => {next}"
+  | .Union alts =>
+      let lines := String.join (alts.toList |> List.map (fun t => s!" {t}"))
+      s!"Union [{lines} ]"
+  | .UnionReverse alts =>
+      let lines := String.join (alts.toList |> List.map (fun t => s!" {t}"))
+      s!"UnionReverse [{lines} ]"
+  | .BinaryUnion alt1 alt2 => s!"binary-union({alt1}, {alt2})"
+  | .Capture next pattern_id group slot =>
+      s!"capture(pid={pattern_id}, group={group}, slot={slot}) => {next}"
+  | .Match pattern_id => s!"Match({pattern_id})"
+
+end State
+
+instance : ToString $ State n where toString s := Checked.State.toString s
+
+/-- A char oriented Thompson non-deterministic finite automaton (NFA) with n states -/
+structure NFA where
+  /-- number of states -/
+  n : Nat
+  /-- states of the NFA -/
+  states : Array (State n)
+  /-- assertion that n equals size of states -/
+  isEq : n = states.size
+
+instance : Inhabited NFA where default := ⟨0, #[], by simp_arith⟩
+
+instance {nfa : NFA} : Coe (Fin nfa.n) (Fin (Array.size nfa.states)) where
+  coe n := Fin.castLE (by simp[nfa.isEq]) n
+
+def toString (nfa : NFA) : String :=
+  let states := Array.mapIdx nfa.states (fun i s => (i, s))
+  let states := String.join (states.toList |> List.map (fun (i, s) =>
+      let iv := String.mk (Nat.toDigits 10 i.val)
+      "\n  " ++ iv ++ ": " ++ s.toString))
+  s!"states {states}"
+
 instance : ToString NFA where
-  toString := NFA.toString
+  toString := Checked.toString
+
+end Checked
+
+private def toFin? (i n : Nat) : Option $ Fin n :=
+  if h : i < n then some ⟨i, h⟩ else none
+
+private def toCkeckedTransition? (t : Unchecked.Transition) (n : Nat) : Option $ Checked.Transition n :=
+  if h : t.next < n
+  then some $ ⟨t.start, t.end, ⟨t.next, h⟩⟩
+  else none
+
+private def toCkeckedState? (s : Unchecked.State) (n : Nat) : Option $ Checked.State n :=
+  match s with
+  | .Empty next => (toFin? next n) |> Option.map (Checked.State.Empty ·)
+  | .ByteRange trans => (toCkeckedTransition? trans n) |> Option.map (Checked.State.ByteRange ·)
+  | .SparseTransitions trans =>
+        trans
+        |> Array.mapM (fun t => toCkeckedTransition? t n)
+        |> Option.map (fun trans => (Checked.State.SparseTransitions trans))
+
+  | .Look look next => (toFin? next n) |> Option.map (Checked.State.Look look ·)
+  | .Union alts =>
+        alts
+        |> Array.mapM (fun alt => toFin? alt n)
+        |> Option.map (fun alts => (Checked.State.Union alts))
+  | .UnionReverse alts =>
+        alts
+        |> Array.mapM (fun alt => toFin? alt n)
+        |> Option.map (fun alts => (Checked.State.UnionReverse alts))
+  | .BinaryUnion alt1 alt2 =>
+        match (toFin? alt1 n), (toFin? alt2 n) with
+        | some alt1, some alt2 => (Checked.State.BinaryUnion alt1 alt2)
+        | _, _ => none
+  | .Capture next pattern_id group slot =>
+        (toFin? next n) |> Option.map (Checked.State.Capture · pattern_id group slot)
+  | .Match pattern_id => some (Checked.State.Match pattern_id)
+
+/-- transform Unchecked.NFA to Checked.NFA -/
+def toCkecked (nfa : Unchecked.NFA) : Except String $ Checked.NFA :=
+  let n := nfa.states.size
+  match nfa.states |> Array.mapM (toCkeckedState? · n) with
+  | some states =>
+    if h : nfa.states.size = states.size -- todo: prove it
+    then Except.ok ⟨n, states, by simp_all⟩
+    else Except.error "internal error: NFA.toCkecked failed"
+  | none => Except.error "internal error: NFA.toCkecked failed"
